src/3d/InterpreterTarget.fst
@@ -1,0 +1,387 @@
+(*
+   Copyright 2019 Microsoft Research
+
+   Licensed under the Apache License, Version 2.0 (the "License");
+   you may not use this file except in compliance with the License.
+   You may obtain a copy of the License at
+
+       http://www.apache.org/licenses/LICENSE-2.0
+
+   Unless required by applicable law or agreed to in writing, software
+   distributed under the License is distributed on an "AS IS" BASIS,
+   WITHOUT WARRANTIES OR CONDITIONS OF ANY KIND, either express or implied.
+   See the License for the specific language governing permissions and
+   limitations under the License.
+*)
+module InterpreterTarget
+(* The abstract syntax for the code produced by 3d, targeting prelude/Interpreter.fst *)
+open FStar.All
+module A = Ast
+module T = Target
+open Binding
+
+let expr = T.expr
+let action = T.action
+let lam a = A.ident & a
+type itype =
+  | UInt8
+  | UInt16
+  | UInt32
+  | UInt64
+
+noeq
+type dtyp : Type =
+  | DT_IType:
+      i:itype -> dtyp
+
+  | DT_App:
+      hd:A.ident ->
+      args:list expr ->
+      dtyp
+
+noeq
+type typ : Type =
+  | T_false:
+      typ
+
+  | T_denoted:
+      d:dtyp ->
+      typ
+
+  | T_pair:
+      t1:typ ->
+      t2:typ ->
+      typ
+
+  | T_dep_pair:
+      t1:dtyp ->
+      t2:lam typ ->
+      typ
+
+  | T_refine:
+      base:dtyp ->
+      refinement:lam expr ->
+      typ
+
+  | T_dep_pair_with_refinement:
+      base:dtyp ->
+      refinement:lam expr ->
+      k:lam typ ->
+      typ
+
+  | T_dep_pair_with_refinement_and_action:
+      base:dtyp ->
+      refinement:lam expr ->
+      k:lam typ ->
+      a:lam action ->
+      typ
+
+  | T_if_else:
+      b:expr ->
+      t1:typ ->
+      t2:typ ->
+      typ
+
+  | T_with_action:
+      base:typ ->
+      act:action ->
+      typ
+
+  | T_with_dep_action:
+      head:dtyp ->
+      act:lam action ->
+      typ
+
+  | T_with_comment:
+      t:typ ->
+      c:A.comments ->
+      typ
+
+  | T_nlist:
+      n:expr ->
+      t:typ ->
+      typ
+
+  | T_at_most:
+      n:expr ->
+      t:typ ->
+      typ
+
+  | T_exact:
+      n:expr ->
+      t:typ ->
+      typ
+
+  | T_string:
+      element_type:dtyp ->
+      terminator:expr ->
+      typ
+
+let type_decl = A.ident & typ
+
+
+let dtyp_of_app (hd:A.ident) (args:list T.index)
+  : ML dtyp
+  = match hd.v.name, args with
+    | "UINT8", [] ->
+      DT_IType UInt8
+
+    | "UINT16", [] ->
+      DT_IType UInt16
+
+    | "UINT32", [] ->
+      DT_IType UInt32
+
+    | "UINT64", [] ->
+      DT_IType UInt64
+
+    | _ ->
+      failwith (Printf.sprintf "Not yet handled: <%s>" hd.v.name)
+
+let tag_of_parser p
+  = let open T in
+    match p.p_parser with
+    | Parse_return _ -> "Parse_return"
+    | Parse_app _ _ -> "Parse_app"
+    | Parse_nlist _ _ -> "Parse_nlist"
+    | Parse_t_at_most _ _ -> "Parse_t_at_most"
+    | Parse_t_exact _ _ -> "Parse_t_exact"
+    | Parse_pair _ _ _ -> "Parse_pair"
+    | Parse_dep_pair _ _ _ -> "Parse_dep_pair"
+    | Parse_dep_pair_with_refinement _ _ _ _ -> "Parse_dep_pair_with_refinement"
+    | Parse_dep_pair_with_action _ _ _ -> "Parse_dep_pair_with_action"
+    | Parse_dep_pair_with_refinement_and_action _ _ _ _ _ -> "Parse_dep_pair_with_refinement_and_action"
+    | Parse_map _ _ -> "Parse_map"
+    | Parse_refinement _ _ _ -> "Parse_refinement"
+    | Parse_refinement_with_action _ _ _ _ -> "Parse_refinement_with_action"
+    | Parse_with_dep_action _ _ _ -> "Parse_with_dep_action"
+    | Parse_with_action _ _ _ -> "Parse_with_action"
+    | Parse_weaken_left _ _ -> "Parse_weaken_left"
+    | Parse_weaken_right _ _ -> "Parse_weaken_right"
+    | Parse_if_else _ _ _ -> "Parse_if_else"
+    | Parse_impos -> "Parse_impos"
+    | Parse_with_comment _ _ -> "Parse_with_comment"
+    | Parse_string _ _ -> "Parse_string"
+
+let as_lam (x:T.lam 'a)
+  : lam 'a
+  = let i =
+      match fst x with
+      | None -> A.(with_dummy_range (to_ident' "_"))
+      | Some i -> i
+    in
+    i, snd x
+
+let rec typ_of_parser (p:T.parser)
+  : ML typ
+  = let dtyp_of_parser (p:T.parser)
+      : ML dtyp
+      = match p.p_parser with
+        | T.Parse_app hd args ->
+          dtyp_of_app hd args
+        | _ ->
+          failwith "Expected a named type"
+    in
+    match p.p_parser with
+    | T.Parse_impos ->
+      T_false
+
+    | T.Parse_app _ _ ->
+      T_denoted (dtyp_of_parser p)
+
+    | T.Parse_pair _ p q ->
+      T_pair (typ_of_parser p) (typ_of_parser q)
+
+    | T.Parse_with_comment p c ->
+      T_with_comment (typ_of_parser p) c
+
+    | T.Parse_nlist n p ->
+      T_nlist n (typ_of_parser p)
+
+    | T.Parse_t_at_most n p ->
+      T_at_most n (typ_of_parser p)
+
+    | T.Parse_t_exact n p ->
+      T_exact n (typ_of_parser p)
+
+    | T.Parse_if_else e p1 p2 ->
+      T_if_else e (typ_of_parser p1) (typ_of_parser p2)
+
+    | T.Parse_dep_pair _ p k ->
+      let i, k = as_lam k in
+      T_dep_pair (dtyp_of_parser p)
+                 (i, typ_of_parser k)
+
+    | T.Parse_dep_pair_with_refinement _ p r k ->
+      let i, r = as_lam r in
+      let j, k = as_lam k in
+      T_dep_pair_with_refinement (dtyp_of_parser p) (i, r) (j, typ_of_parser k)
+
+    | T.Parse_dep_pair_with_action p a k ->
+      let a = as_lam a in
+      let (i, k) = as_lam k in
+      let r = as_lam (None, T.mk_expr (T.Constant (A.Bool true))) in
+      T_dep_pair_with_refinement_and_action (dtyp_of_parser p) r (i, typ_of_parser k) a
+
+    | T.Parse_dep_pair_with_refinement_and_action _ p r a k ->
+      let a = as_lam a in
+      let (i, k) = as_lam k in
+      let r = as_lam r in
+      T_dep_pair_with_refinement_and_action (dtyp_of_parser p) r (i, typ_of_parser k) a
+
+    | T.Parse_with_action _ p a ->
+      T_with_action (typ_of_parser p) a
+
+    | T.Parse_with_dep_action _ p a ->
+      let a = as_lam a in
+      T_with_dep_action (dtyp_of_parser p) a
+
+    | T.Parse_string p z ->
+      T_string (dtyp_of_parser p) z
+
+    | T.Parse_refinement _ p f ->
+      T_refine (dtyp_of_parser p) (as_lam f)
+
+    | T.Parse_refinement_with_action _ _ _ _ ->
+      failwith "Not yet implemented"
+
+    | T.Parse_weaken_left _ _
+    | T.Parse_weaken_right _ _
+    | T.Parse_map _ _
+    | T.Parse_return _ -> failwith "Unnecessary"
+
+let translate_decls (ds:T.decls)
+  : ML (list type_decl)
+  = List.collect
+      (function
+        | (T.Type_decl td, _) ->
+          [td.decl_name.td_name, typ_of_parser td.decl_parser]
+        | _ ->
+          [])
+      ds
+
+let print_ityp (i:itype) =
+  match i with
+  | UInt8 -> "UInt8"
+  | UInt16 -> "UInt16"
+  | UInt32 -> "UInt32"
+  | UInt64 -> "UInt64"
+
+let print_ident (mname:string) (i:A.ident) =
+  T.print_maybe_qualified_ident mname i
+
+let print_dtyp (mname:string) (dt:dtyp) =
+  match dt with
+  | DT_IType i ->
+    Printf.sprintf "(DT_IType %s)" (print_ityp i)
+
+  | DT_App hd args ->
+    Printf.sprintf "(DT_App %s %s)"
+      (print_ident mname hd)
+      (List.map (T.print_expr mname) args |> String.concat " ")
+
+let print_lam (p:'a -> ML string) (x:lam 'a) =
+  Printf.sprintf "(fun %s -> %s)"
+    (fst x).v.name
+    (p (snd x))
+
+let rec print_typ (mname:string) (t:typ)
+  : ML string
+  = match t with
+    | T_false ->
+      "T_false"
+
+    | T_denoted dt ->
+      print_dtyp mname dt
+
+    | T_pair t1 t2 ->
+      Printf.sprintf "(T_pair %s %s)"
+                     (print_typ mname t1)
+                     (print_typ mname t2)
+
+    | T_dep_pair t k ->
+      Printf.sprintf "(T_dep_pair %s %s)"
+                     (print_dtyp mname t)
+                     (print_lam (print_typ mname) k)
+
+    | T_refine d r ->
+      Printf.sprintf "(T_refine %s %s)"
+                     (print_dtyp mname d)
+                     (print_lam (T.print_expr mname) r)
+
+
+    | T_dep_pair_with_refinement d r k ->
+      Printf.sprintf "(T_dep_pair_with_refinement %s %s %s)"
+                     (print_dtyp mname d)
+                     (print_lam (T.print_expr mname) r)
+                     (print_lam (print_typ mname) k)
+
+    | T_dep_pair_with_refinement_and_action d r k a ->
+      Printf.sprintf "(T_dep_pair_with_refinement_and_action %s %s %s %s)"
+                     (print_dtyp mname d)
+                     (print_lam (T.print_expr mname) r)
+                     (print_lam (print_typ mname) k)
+                     (print_lam (T.print_action mname) a)
+
+    | T_if_else e t1 t2 ->
+      Printf.sprintf "(T_if_else %s %s %s)"
+                     (T.print_expr mname e)
+                     (print_typ mname t1)
+                     (print_typ mname t2)
+
+    | T_with_action p a ->
+      Printf.sprintf "(T_with_action %s %s)"
+                     (print_typ mname p)
+                     (T.print_action mname a)
+
+    | T_with_dep_action d a ->
+      Printf.sprintf "(T_with_dep_action %s %s)"
+                     (print_dtyp mname d)
+                     (print_lam (T.print_action mname) a)
+
+    | T_with_comment t c ->
+      Printf.sprintf "(T_with_comment %s [%s])"
+                     (print_typ mname t)
+                     (List.map (Printf.sprintf "\"%s\"") c |> String.concat "; ")
+
+    | T_nlist n t ->
+      Printf.sprintf "(T_nlist %s %s)"
+                     (T.print_expr mname n)
+                     (print_typ mname t)
+
+    | T_at_most n t ->
+      Printf.sprintf "(T_at_most %s %s)"
+                     (T.print_expr mname n)
+                     (print_typ mname t)
+
+    | T_exact n t ->
+      Printf.sprintf "(T_exact %s %s)"
+                     (T.print_expr mname n)
+                     (print_typ mname t)
+
+    | T_string d z ->
+      Printf.sprintf "(T_string %s %s)"
+                     (print_dtyp mname d)
+                     (T.print_expr mname z)
+
+let print_type_decl mname (td:type_decl) =
+  FStar.Printf.sprintf
+    "[@@specialize]\n
+     let %s = %s\n"
+      (fst td).v.name
+      (print_typ mname (snd td))
+
+let print_type_decls mname tds =
+  List.map (print_type_decl mname) tds |>
+  String.concat "\n\n"
+
+let print_validator (td:type_decl) =
+  FStar.Printf.sprintf
+    "[@@T.postprocess_for_extraction_with specialize_tac]\n
+     let validate_%s = as_validator %s\n"
+      (fst td).v.name
+      (fst td).v.name
+
+let print_validators mname tds =
+  List.map print_validator tds |>
+  String.concat "\n\n"
