src/3d/InterpreterTarget.fsti
@@ -1,0 +1,32 @@
+(*
+   Copyright 2019 Microsoft Research
+
+   Licensed under the Apache License, Version 2.0 (the "License");
+   you may not use this file except in compliance with the License.
+   You may obtain a copy of the License at
+
+       http://www.apache.org/licenses/LICENSE-2.0
+
+   Unless required by applicable law or agreed to in writing, software
+   distributed under the License is distributed on an "AS IS" BASIS,
+   WITHOUT WARRANTIES OR CONDITIONS OF ANY KIND, either express or implied.
+   See the License for the specific language governing permissions and
+   limitations under the License.
+*)
+module InterpreterTarget
+(* The abstract syntax for the code produced by 3d, targeting prelude/Interpreter.fst *)
+open FStar.All
+module A = Ast
+module T = Target
+open Binding
+
+val type_decl : Type0
+
+val translate_decls (ds:T.decls)
+  : ML (list type_decl)
+
+val print_type_decls (mname:string) (ds:list type_decl)
+  : ML string
+
+val print_validators (mname:string) (ds:list type_decl)
+  : ML string
