src/3d/Target.fsti
@@ -397,7 +397,11 @@ type decl = decl' * decl_attributes
 type decls = list decl
 
 val error_handler_decl : decl
+val print_maybe_qualified_ident (mname:string) (i:A.ident) : ML string
+val print_expr (mname:string) (e:expr) : ML string
 val print_typ (mname:string) (t:typ) : ML string //(decreases t)
+val print_parser (mname:string) (p:parser) : ML string
+val print_action (mname:string) (a:action) : ML string
 val print_decls (modul: string) (ds:list decl) : ML string
 val print_types_decls (modul: string) (ds:list decl) : ML string
 val print_decls_signature (modul: string) (ds:list decl) : ML string
